<?xml version="1.0"?>
<rdf:RDF xmlns="http://purl.obolibrary.org/obo/obi/dev/import/ENVO_imports.owl#"
     xml:base="http://purl.obolibrary.org/obo/obi/dev/import/ENVO_imports.owl"
     xmlns:obo="http://purl.obolibrary.org/obo/"
     xmlns:owl="http://www.w3.org/2002/07/owl#"
     xmlns:rdf="http://www.w3.org/1999/02/22-rdf-syntax-ns#"
     xmlns:xml="http://www.w3.org/XML/1998/namespace"
     xmlns:xsd="http://www.w3.org/2001/XMLSchema#"
     xmlns:rdfs="http://www.w3.org/2000/01/rdf-schema#"
     xmlns:oboInOwl="http://www.geneontology.org/formats/oboInOwl#">
    <owl:Ontology rdf:about="http://purl.obolibrary.org/obo/obi/dev/import/ENVO_imports.owl"/>
    


    <!-- 
    ///////////////////////////////////////////////////////////////////////////////////////
    //
    // Annotation properties
    //
    ///////////////////////////////////////////////////////////////////////////////////////
     -->

    


    <!-- http://purl.obolibrary.org/obo/IAO_0000115 -->

    <owl:AnnotationProperty rdf:about="http://purl.obolibrary.org/obo/IAO_0000115">
        <rdfs:label>definition</rdfs:label>
    </owl:AnnotationProperty>
    


    <!-- http://purl.obolibrary.org/obo/IAO_0000116 -->

    <owl:AnnotationProperty rdf:about="http://purl.obolibrary.org/obo/IAO_0000116">
        <rdfs:label>editor note</rdfs:label>
    </owl:AnnotationProperty>
    


    <!-- http://www.geneontology.org/formats/oboInOwl#hasBroadSynonym -->

    <owl:AnnotationProperty rdf:about="http://www.geneontology.org/formats/oboInOwl#hasBroadSynonym">
        <rdfs:label>has_broad_synonym</rdfs:label>
    </owl:AnnotationProperty>
    


    <!-- http://www.geneontology.org/formats/oboInOwl#hasDbXref -->

    <owl:AnnotationProperty rdf:about="http://www.geneontology.org/formats/oboInOwl#hasDbXref">
        <rdfs:label>database_cross_reference</rdfs:label>
    </owl:AnnotationProperty>
    


    <!-- http://www.geneontology.org/formats/oboInOwl#hasExactSynonym -->

    <owl:AnnotationProperty rdf:about="http://www.geneontology.org/formats/oboInOwl#hasExactSynonym">
        <rdfs:label>has_exact_synonym</rdfs:label>
    </owl:AnnotationProperty>
    


    <!-- http://www.geneontology.org/formats/oboInOwl#hasRelatedSynonym -->

    <owl:AnnotationProperty rdf:about="http://www.geneontology.org/formats/oboInOwl#hasRelatedSynonym">
        <rdfs:label>has_related_synonym</rdfs:label>
    </owl:AnnotationProperty>
    


    <!-- http://www.geneontology.org/formats/oboInOwl#inSubset -->

    <owl:AnnotationProperty rdf:about="http://www.geneontology.org/formats/oboInOwl#inSubset">
        <rdfs:label>in_subset</rdfs:label>
    </owl:AnnotationProperty>
    


    <!-- 
    ///////////////////////////////////////////////////////////////////////////////////////
    //
    // Classes
    //
    ///////////////////////////////////////////////////////////////////////////////////////
     -->

    


    <!-- http://purl.obolibrary.org/obo/BFO_0000040 -->

    <owl:Class rdf:about="http://purl.obolibrary.org/obo/BFO_0000040">
        <obo:IAO_0000115 xml:lang="en">An independent continuant that is spatially extended whose identity is independent of that of other entities and can be maintained through time.</obo:IAO_0000115>
        <rdfs:label xml:lang="en">material entity</rdfs:label>
    </owl:Class>
    


    <!-- http://purl.obolibrary.org/obo/ENVO_00001998 -->

    <owl:Class rdf:about="http://purl.obolibrary.org/obo/ENVO_00001998">
        <rdfs:subClassOf rdf:resource="http://purl.obolibrary.org/obo/ENVO_00010483"/>
        <obo:IAO_0000115 xml:lang="en">An environmental material which is primarily composed of minerals, varying proportions of sand, silt, and clay, organic material such as humus, interstitial gases, liquids, and a broad range of resident micro- and macroorganisms.</obo:IAO_0000115>
        <obo:IAO_0000116>The various &apos;has part&apos; and &apos;has quality&apos; relations may not hold true for all soils; however, I have yet to find counter examples. Require input from a pedologist or similar. [pbuttigieg]</obo:IAO_0000116>
        <oboInOwl:hasBroadSynonym>regolith</oboInOwl:hasBroadSynonym>
        <oboInOwl:hasDbXref>LTER:535</oboInOwl:hasDbXref>
        <oboInOwl:hasDbXref>SPIRE:Soil</oboInOwl:hasDbXref>
        <oboInOwl:hasDbXref>SWEETRealm:Soil</oboInOwl:hasDbXref>
        <oboInOwl:hasDbXref>https://en.wikipedia.org/wiki/Soil</oboInOwl:hasDbXref>
        <oboInOwl:inSubset rdf:resource="http://purl.obolibrary.org/obo/ENVO_03605015"/>
        <oboInOwl:inSubset rdf:resource="http://purl.obolibrary.org/obo/envo#EnvO-Lite-GSC"/>
        <rdfs:comment>&apos;In engineering terms, soil is referred to as regolith, or loose rock material that lies above the &apos;solid geology&apos;. Soil is commonly referred to as &quot;earth&quot; or &quot;dirt&quot;; technically, the term &quot;dirt&quot; should be restricted to displaced soil.&apos; https://en.wikipedia.org/wiki/Soil

&quot; The upper limit of soil is the boundary between soil and air, shallow water, live plants, or plant materials that have not begun to decompose. Areas are not considered to have soil if the surface is permanently covered by water too deep (typically more than 2.5 meters) for the growth of rooted plants.

The lower boundary that separates soil from the nonsoil underneath is most difficult to define. Soil consists of horizons near the Earth&apos;s surface that, in contrast to the underlying parent material, have been altered by the interactions of climate, relief, and living organisms over time. Commonly, soil grades at its lower boundary to hard rock or to earthy materials virtually devoid of animals, roots, or other marks of biological activity. For purposes of classification, the lower boundary of soil is arbitrarily set at 200 cm.&quot;  Soil taxonomy, 2nd Ed., quoted in http://www.nrcs.usda.gov/wps/portal/nrcs/detail/soils/edu/?cid=nrcs142p2_054280</rdfs:comment>
        <rdfs:label>soil</rdfs:label>
    </owl:Class>
    <owl:Axiom>
        <owl:annotatedSource rdf:resource="http://purl.obolibrary.org/obo/ENVO_00001998"/>
        <owl:annotatedProperty rdf:resource="http://purl.obolibrary.org/obo/IAO_0000115"/>
        <owl:annotatedTarget xml:lang="en">An environmental material which is primarily composed of minerals, varying proportions of sand, silt, and clay, organic material such as humus, interstitial gases, liquids, and a broad range of resident micro- and macroorganisms.</owl:annotatedTarget>
        <oboInOwl:hasDbXref>https://en.wikipedia.org/wiki/Soil</oboInOwl:hasDbXref>
    </owl:Axiom>
    


    <!-- http://purl.obolibrary.org/obo/ENVO_00002257 -->

    <owl:Class rdf:about="http://purl.obolibrary.org/obo/ENVO_00002257">
        <rdfs:subClassOf rdf:resource="http://purl.obolibrary.org/obo/ENVO_00001998"/>
        <obo:IAO_0000115>Podzols are soils with a typically ash-grey upper subsurface horizon, bleached by loss of organic matter and iron oxides, on top of a dark accumulation horizon with brown, reddish or black illuviated humus and/or reddish Fe compounds. Podzols occur in humid areas in the boreal and temperate zones and locally also in the tropics.</obo:IAO_0000115>
        <oboInOwl:hasDbXref>https://en.wikipedia.org/wiki/Podzol</oboInOwl:hasDbXref>
        <oboInOwl:hasExactSynonym>podsol</oboInOwl:hasExactSynonym>
        <oboInOwl:hasRelatedSynonym>podosolic soil</oboInOwl:hasRelatedSynonym>
        <oboInOwl:inSubset rdf:resource="http://purl.obolibrary.org/obo/ENVO_03605015"/>
        <rdfs:label>podzol</rdfs:label>
    </owl:Class>
    <owl:Axiom>
        <owl:annotatedSource rdf:resource="http://purl.obolibrary.org/obo/ENVO_00002257"/>
        <owl:annotatedProperty rdf:resource="http://purl.obolibrary.org/obo/IAO_0000115"/>
        <owl:annotatedTarget>Podzols are soils with a typically ash-grey upper subsurface horizon, bleached by loss of organic matter and iron oxides, on top of a dark accumulation horizon with brown, reddish or black illuviated humus and/or reddish Fe compounds. Podzols occur in humid areas in the boreal and temperate zones and locally also in the tropics.</owl:annotatedTarget>
        <oboInOwl:hasDbXref>http://fao.org/ag/agl/agll/wrb/doc/wrb2006final.pdf</oboInOwl:hasDbXref>
    </owl:Axiom>
    


    <!-- http://purl.obolibrary.org/obo/ENVO_00010483 -->

    <owl:Class rdf:about="http://purl.obolibrary.org/obo/ENVO_00010483">
        <rdfs:subClassOf rdf:resource="http://purl.obolibrary.org/obo/BFO_0000040"/>
        <obo:IAO_0000115 xml:lang="en">A material entity which other material entities in an environmental system are primarily or partially composed of.</obo:IAO_0000115>
        <oboInOwl:hasExactSynonym>portion of environmental material</oboInOwl:hasExactSynonym>
        <rdfs:comment xml:lang="en">Everything under this parent must be a mass noun (i.e. not countable). All subclasses are to be understood as being composed primarily of the named entity, rather than restricted to that entity. For example, &quot;ENVO:water&quot; is to be understood as &quot;environmental material composed primarly of some CHEBI:water&quot;.</rdfs:comment>
        <rdfs:comment xml:lang="en">Instances of this class are portions of environmental materials, such as seawater in bucket, a water parcel in the photic zone of a lake, or the concrete that composes a building part. Instances of these portions may have fiat or non-fiat boundaries. For example, a water parcel has not physical boundaries, while the seawater in a bucket is bounded by the internal surfaces of the bucket.</rdfs:comment>
        <rdfs:label>environmental material</rdfs:label>
    </owl:Class>
    <owl:Axiom>
        <owl:annotatedSource rdf:resource="http://purl.obolibrary.org/obo/ENVO_00010483"/>
        <owl:annotatedProperty rdf:resource="http://purl.obolibrary.org/obo/IAO_0000115"/>
        <owl:annotatedTarget xml:lang="en">A material entity which other material entities in an environmental system are primarily or partially composed of.</owl:annotatedTarget>
        <oboInOwl:hasDbXref rdf:resource="http://ontology.buffalo.edu/smith/articles/niches.html"/>
        <oboInOwl:hasDbXref rdf:resource="https://dx.doi.org/10.1186/2041-1480-4-43"/>
        <oboInOwl:hasDbXref rdf:resource="https://en.wikipedia.org/wiki/Material"/>
    </owl:Axiom>
</rdf:RDF>



<!-- Generated by the OWL API (version 4.5.25) https://github.com/owlcs/owlapi -->

