<?xml version="1.0"?>
<rdf:RDF xmlns="http://purl.obolibrary.org/obo/obi/dev/import/FOODON_imports.owl#"
     xml:base="http://purl.obolibrary.org/obo/obi/dev/import/FOODON_imports.owl"
     xmlns:obo="http://purl.obolibrary.org/obo/"
     xmlns:owl="http://www.w3.org/2002/07/owl#"
     xmlns:rdf="http://www.w3.org/1999/02/22-rdf-syntax-ns#"
     xmlns:xml="http://www.w3.org/XML/1998/namespace"
     xmlns:xsd="http://www.w3.org/2001/XMLSchema#"
     xmlns:rdfs="http://www.w3.org/2000/01/rdf-schema#">
    <owl:Ontology rdf:about="http://purl.obolibrary.org/obo/obi/dev/import/FOODON_imports.owl"/>
    


    <!-- 
    ///////////////////////////////////////////////////////////////////////////////////////
    //
    // Annotation properties
    //
    ///////////////////////////////////////////////////////////////////////////////////////
     -->

    


    <!-- http://purl.obolibrary.org/obo/IAO_0000111 -->

    <owl:AnnotationProperty rdf:about="http://purl.obolibrary.org/obo/IAO_0000111">
        <obo:IAO_0000111>editor preferred label</obo:IAO_0000111>
        <obo:IAO_0000111 xml:lang="en">editor preferred label</obo:IAO_0000111>
        <obo:IAO_0000111>editor preferred term</obo:IAO_0000111>
        <obo:IAO_0000111 xml:lang="en">editor preferred term</obo:IAO_0000111>
        <obo:IAO_0000111>editor preferred term~editor preferred label</obo:IAO_0000111>
        <obo:IAO_0000115 xml:lang="en">The concise, meaningful, and human-friendly name for a class or property preferred by the ontology developers. (US-English)</obo:IAO_0000115>
        <rdfs:label>editor preferred label</rdfs:label>
        <rdfs:label xml:lang="en">editor preferred label</rdfs:label>
        <rdfs:label>editor preferred term</rdfs:label>
        <rdfs:label xml:lang="en">editor preferred term</rdfs:label>
        <rdfs:label>editor preferred term~editor preferred label</rdfs:label>
    </owl:AnnotationProperty>
    


    <!-- http://purl.obolibrary.org/obo/IAO_0000115 -->

    <owl:AnnotationProperty rdf:about="http://purl.obolibrary.org/obo/IAO_0000115">
        <obo:IAO_0000111>definition</obo:IAO_0000111>
        <obo:IAO_0000111 xml:lang="en">definition</obo:IAO_0000111>
        <obo:IAO_0000111>textual definition</obo:IAO_0000111>
        <obo:IAO_0000115>A property representing the English language definitions of what NCI means by the concept. They may also include information about the definition&apos;s source and attribution in a form that can easily be interpreted by software.</obo:IAO_0000115>
        <obo:IAO_0000115>English language definitions of what NCI means by the concept. These are limited to 1024 characters. They may also include information about the definition&apos;s source and attribution in a form that can easily be interpreted by software.</obo:IAO_0000115>
        <obo:IAO_0000115 xml:lang="en">The official OBI definition, explaining the meaning of a class or property. Shall be Aristotelian, formalized and normalized. Can be augmented with colloquial definitions.</obo:IAO_0000115>
        <obo:IAO_0000115 xml:lang="en">The official definition, explaining the meaning of a class or property. Shall be Aristotelian, formalized and normalized. Can be augmented with colloquial definitions.</obo:IAO_0000115>
        <rdfs:label>definition</rdfs:label>
        <rdfs:label xml:lang="en">definition</rdfs:label>
        <rdfs:label>textual definition</rdfs:label>
    </owl:AnnotationProperty>
    


    <!-- http://purl.obolibrary.org/obo/IAO_0000412 -->

    <owl:AnnotationProperty rdf:about="http://purl.obolibrary.org/obo/IAO_0000412">
        <rdfs:label xml:lang="en">imported from</rdfs:label>
    </owl:AnnotationProperty>
    


    <!-- http://www.w3.org/2000/01/rdf-schema#label -->

    <owl:AnnotationProperty rdf:about="http://www.w3.org/2000/01/rdf-schema#label">
        <obo:IAO_0000111>label</obo:IAO_0000111>
        <obo:IAO_0000111 xml:lang="en">label</obo:IAO_0000111>
        <rdfs:label>label</rdfs:label>
        <rdfs:label xml:lang="en">label</rdfs:label>
    </owl:AnnotationProperty>
    


    <!-- 
    ///////////////////////////////////////////////////////////////////////////////////////
    //
    // Classes
    //
    ///////////////////////////////////////////////////////////////////////////////////////
     -->

    


    <!-- http://purl.obolibrary.org/obo/BFO_0000040 -->

    <owl:Class rdf:about="http://purl.obolibrary.org/obo/BFO_0000040"/>
    


    <!-- http://purl.obolibrary.org/obo/FOODON_00002147 -->

    <owl:Class rdf:about="http://purl.obolibrary.org/obo/FOODON_00002147">
        <rdfs:subClassOf rdf:resource="http://purl.obolibrary.org/obo/FOODON_00002403"/>
        <obo:IAO_0000111 xml:lang="en">food material by consumer group</obo:IAO_0000111>
        <obo:IAO_0000412 rdf:resource="http://purl.obolibrary.org/obo/foodon.owl"/>
        <rdfs:label xml:lang="en">food material by consumer group</rdfs:label>
    </owl:Class>
    


    <!-- http://purl.obolibrary.org/obo/FOODON_00002403 -->

    <owl:Class rdf:about="http://purl.obolibrary.org/obo/FOODON_00002403">
        <rdfs:subClassOf rdf:resource="http://purl.obolibrary.org/obo/BFO_0000040"/>
        <obo:IAO_0000111 xml:lang="en">food material</obo:IAO_0000111>
        <obo:IAO_0000115 xml:lang="en">Any substance that can be consumed by an organism to satisfy nutritional or other health needs, or to provide a social or organoleptic food experience</obo:IAO_0000115>
        <obo:IAO_0000412 rdf:resource="http://purl.obolibrary.org/obo/foodon.owl"/>
        <rdfs:label xml:lang="en">food material</rdfs:label>
    </owl:Class>
    


    <!-- http://purl.obolibrary.org/obo/FOODON_00004325 -->

    <owl:Class rdf:about="http://purl.obolibrary.org/obo/FOODON_00004325">
        <rdfs:subClassOf rdf:resource="http://purl.obolibrary.org/obo/FOODON_03309997"/>
        <obo:IAO_0000111>animal feed</obo:IAO_0000111>
        <obo:IAO_0000115>Food material which can be used to meet nutritional requirements of animals, particularly livestock such as cattle, goats, sheep, horses, chickens and pigs.</obo:IAO_0000115>
        <obo:IAO_0000412 rdf:resource="http://purl.obolibrary.org/obo/foodon.owl"/>
        <rdfs:label>animal feed</rdfs:label>
    </owl:Class>
    


    <!-- http://purl.obolibrary.org/obo/FOODON_03309997 -->

    <owl:Class rdf:about="http://purl.obolibrary.org/obo/FOODON_03309997">
        <rdfs:subClassOf rdf:resource="http://purl.obolibrary.org/obo/FOODON_00002147"/>
        <obo:IAO_0000111 xml:lang="en">food material for animals</obo:IAO_0000111>
        <obo:IAO_0000115 xml:lang="en">Food product for animal covers foods intended for consumption by domesticated animals.</obo:IAO_0000115>
        <obo:IAO_0000412 rdf:resource="http://purl.obolibrary.org/obo/foodon.owl"/>
        <rdfs:label xml:lang="en">food material for animals</rdfs:label>
    </owl:Class>
</rdf:RDF>



<!-- Generated by the OWL API (version 4.5.29) https://github.com/owlcs/owlapi -->

