<?xml version="1.0"?>
<rdf:RDF xmlns="http://purl.obolibrary.org/obo/obi/dev/import/uo_imports.owl#"
     xml:base="http://purl.obolibrary.org/obo/obi/dev/import/uo_imports.owl"
     xmlns:obo="http://purl.obolibrary.org/obo/"
     xmlns:owl="http://www.w3.org/2002/07/owl#"
     xmlns:rdf="http://www.w3.org/1999/02/22-rdf-syntax-ns#"
     xmlns:xml="http://www.w3.org/XML/1998/namespace"
     xmlns:xsd="http://www.w3.org/2001/XMLSchema#"
     xmlns:rdfs="http://www.w3.org/2000/01/rdf-schema#"
     xmlns:oboInOwl="oboInOwl:">
    <owl:Ontology rdf:about="http://purl.obolibrary.org/obo/obi/dev/import/uo_imports.owl"/>
    


    <!-- 
    ///////////////////////////////////////////////////////////////////////////////////////
    //
    // Annotation properties
    //
    ///////////////////////////////////////////////////////////////////////////////////////
     -->

    


    <!-- http://purl.obolibrary.org/obo/IAO_0000111 -->

    <owl:AnnotationProperty rdf:about="http://purl.obolibrary.org/obo/IAO_0000111"/>
    


    <!-- http://purl.obolibrary.org/obo/IAO_0000412 -->

    <owl:AnnotationProperty rdf:about="http://purl.obolibrary.org/obo/IAO_0000412"/>
    


    <!-- oboInOwl:hasExactSynonym -->

    <owl:AnnotationProperty rdf:about="oboInOwl:hasExactSynonym"/>
    


    <!-- 
    ///////////////////////////////////////////////////////////////////////////////////////
    //
    // Classes
    //
    ///////////////////////////////////////////////////////////////////////////////////////
     -->

    


    <!-- http://purl.obolibrary.org/obo/IAO_0000003 -->

    <owl:Class rdf:about="http://purl.obolibrary.org/obo/IAO_0000003"/>
    


    <!-- http://purl.obolibrary.org/obo/UO_0000001 -->

    <owl:Class rdf:about="http://purl.obolibrary.org/obo/UO_0000001">
        <rdfs:subClassOf rdf:resource="http://purl.obolibrary.org/obo/IAO_0000003"/>
        <obo:IAO_0000111>length unit</obo:IAO_0000111>
        <obo:IAO_0000412 rdf:resource="http://purl.obolibrary.org/obo/uo.owl"/>
        <rdfs:comment>&quot;A unit which is a standard measure of the distance between two points.&quot; [Wikipedia:Wikipedia]</rdfs:comment>
        <rdfs:label>length unit</rdfs:label>
    </owl:Class>
    


    <!-- http://purl.obolibrary.org/obo/UO_0000002 -->

    <owl:Class rdf:about="http://purl.obolibrary.org/obo/UO_0000002">
        <rdfs:subClassOf rdf:resource="http://purl.obolibrary.org/obo/IAO_0000003"/>
        <obo:IAO_0000111>mass unit</obo:IAO_0000111>
        <obo:IAO_0000412 rdf:resource="http://purl.obolibrary.org/obo/uo.owl"/>
        <rdfs:comment>&quot;A unit which is a standard measure of the amount of matter/energy of a physical object.&quot; [Wikipedia:Wikipedia]</rdfs:comment>
        <rdfs:label>mass unit</rdfs:label>
    </owl:Class>
    


    <!-- http://purl.obolibrary.org/obo/UO_0000003 -->

    <owl:Class rdf:about="http://purl.obolibrary.org/obo/UO_0000003">
        <rdfs:subClassOf rdf:resource="http://purl.obolibrary.org/obo/IAO_0000003"/>
        <obo:IAO_0000111>time unit</obo:IAO_0000111>
        <obo:IAO_0000412 rdf:resource="http://purl.obolibrary.org/obo/uo.owl"/>
        <rdfs:comment>&quot;A unit which is a standard measure of the dimension in which events occur in sequence.&quot; [Wikipedia:Wikipedia]</rdfs:comment>
        <rdfs:label>time unit</rdfs:label>
        <oboInOwl:hasExactSynonym>time derived unit</oboInOwl:hasExactSynonym>
    </owl:Class>
    


    <!-- http://purl.obolibrary.org/obo/UO_0000005 -->

    <owl:Class rdf:about="http://purl.obolibrary.org/obo/UO_0000005">
        <rdfs:subClassOf rdf:resource="http://purl.obolibrary.org/obo/IAO_0000003"/>
        <obo:IAO_0000111>temperature unit</obo:IAO_0000111>
        <obo:IAO_0000412 rdf:resource="http://purl.obolibrary.org/obo/uo.owl"/>
        <rdfs:comment>&quot;A unit which is a standard measure of the average kinetic energy of the particles in a sample of matter.&quot; [Wikipedia:Wikipedia]</rdfs:comment>
        <rdfs:label>temperature unit</rdfs:label>
        <oboInOwl:hasExactSynonym>temperature derived unit</oboInOwl:hasExactSynonym>
    </owl:Class>
    


    <!-- http://purl.obolibrary.org/obo/UO_0000006 -->

    <owl:Class rdf:about="http://purl.obolibrary.org/obo/UO_0000006">
        <rdfs:subClassOf rdf:resource="http://purl.obolibrary.org/obo/IAO_0000003"/>
        <obo:IAO_0000111>substance unit</obo:IAO_0000111>
        <obo:IAO_0000412 rdf:resource="http://purl.obolibrary.org/obo/uo.owl"/>
        <rdfs:comment>&quot;A unit which is a standardised quantity of an element or compound with uniform composition.&quot; [Wikipedia:Wikipedia]</rdfs:comment>
        <rdfs:label>substance unit</rdfs:label>
    </owl:Class>
    


    <!-- http://purl.obolibrary.org/obo/UO_0000051 -->

    <owl:Class rdf:about="http://purl.obolibrary.org/obo/UO_0000051">
        <rdfs:subClassOf rdf:resource="http://purl.obolibrary.org/obo/IAO_0000003"/>
        <obo:IAO_0000111>concentration unit</obo:IAO_0000111>
        <obo:IAO_0000412 rdf:resource="http://purl.obolibrary.org/obo/uo.owl"/>
        <rdfs:comment>&quot;A unit which represents a standard measurement of how much of a given substance there is mixed with another substance.&quot; [UOC:GVG]</rdfs:comment>
        <rdfs:label>concentration unit</rdfs:label>
    </owl:Class>
    


    <!-- http://purl.obolibrary.org/obo/UO_0000095 -->

    <owl:Class rdf:about="http://purl.obolibrary.org/obo/UO_0000095">
        <rdfs:subClassOf rdf:resource="http://purl.obolibrary.org/obo/IAO_0000003"/>
        <obo:IAO_0000111>volume unit</obo:IAO_0000111>
        <obo:IAO_0000412 rdf:resource="http://purl.obolibrary.org/obo/uo.owl"/>
        <rdfs:comment>&quot;A unit which is a standard measure of the amount of space occupied by any substance, whether solid, liquid, or gas.&quot; [NIST:NIST]</rdfs:comment>
        <rdfs:label>volume unit</rdfs:label>
    </owl:Class>
    


    <!-- http://purl.obolibrary.org/obo/UO_0000105 -->

    <owl:Class rdf:about="http://purl.obolibrary.org/obo/UO_0000105">
        <rdfs:subClassOf rdf:resource="http://purl.obolibrary.org/obo/IAO_0000003"/>
        <obo:IAO_0000111>frequency unit</obo:IAO_0000111>
        <obo:IAO_0000412 rdf:resource="http://purl.obolibrary.org/obo/uo.owl"/>
        <rdfs:comment>&quot;A unit which is a standard measure of the number of repetitive actions in a particular time.&quot; [NIST:NIST]</rdfs:comment>
        <rdfs:label>frequency unit</rdfs:label>
    </owl:Class>
    


    <!-- http://purl.obolibrary.org/obo/UO_0000109 -->

    <owl:Class rdf:about="http://purl.obolibrary.org/obo/UO_0000109">
        <rdfs:subClassOf rdf:resource="http://purl.obolibrary.org/obo/IAO_0000003"/>
        <obo:IAO_0000111>pressure unit</obo:IAO_0000111>
        <obo:IAO_0000412 rdf:resource="http://purl.obolibrary.org/obo/uo.owl"/>
        <rdfs:comment>&quot;A unit which is a standard measure of the force applied to a given area.&quot; [NIST:NIST]</rdfs:comment>
        <rdfs:label>pressure unit</rdfs:label>
    </owl:Class>
    


    <!-- http://purl.obolibrary.org/obo/UO_0000212 -->

    <owl:Class rdf:about="http://purl.obolibrary.org/obo/UO_0000212">
        <rdfs:subClassOf rdf:resource="http://purl.obolibrary.org/obo/UO_0000051"/>
        <obo:IAO_0000111>colony forming unit per volume</obo:IAO_0000111>
        <obo:IAO_0000412 rdf:resource="http://purl.obolibrary.org/obo/uo.owl"/>
        <rdfs:comment>&quot;A concentration unit which a measure of viable bacterial numbers in a given volume.&quot; [Wikipedia:Wikipedia]</rdfs:comment>
        <rdfs:label>colony forming unit per volume</rdfs:label>
    </owl:Class>
    


    <!-- http://purl.obolibrary.org/obo/UO_0000270 -->

    <owl:Class rdf:about="http://purl.obolibrary.org/obo/UO_0000270">
        <rdfs:subClassOf rdf:resource="http://purl.obolibrary.org/obo/IAO_0000003"/>
        <obo:IAO_0000111>volumetric flow rate unit</obo:IAO_0000111>
        <obo:IAO_0000412 rdf:resource="http://purl.obolibrary.org/obo/uo.owl"/>
        <rdfs:comment>&quot;A unit which is a standard measure of the volume of fluid which passes through a given surface per unit time .&quot; [Wikipedia:Wikipedia]</rdfs:comment>
        <rdfs:label>volumetric flow rate unit</rdfs:label>
    </owl:Class>
    


    <!-- http://purl.obolibrary.org/obo/UO_0000280 -->

    <owl:Class rdf:about="http://purl.obolibrary.org/obo/UO_0000280">
        <rdfs:subClassOf rdf:resource="http://purl.obolibrary.org/obo/IAO_0000003"/>
        <obo:IAO_0000111>rate unit</obo:IAO_0000111>
        <obo:IAO_0000412 rdf:resource="http://purl.obolibrary.org/obo/uo.owl"/>
        <rdfs:comment>&quot;A unit which represents a standard measurement occurrence of a process per unit time.&quot; [UOC:GVG]</rdfs:comment>
        <rdfs:label>rate unit</rdfs:label>
    </owl:Class>
    


    <!-- 
    ///////////////////////////////////////////////////////////////////////////////////////
    //
    // Individuals
    //
    ///////////////////////////////////////////////////////////////////////////////////////
     -->

    


    <!-- http://purl.obolibrary.org/obo/UO_0000008 -->

    <owl:NamedIndividual rdf:about="http://purl.obolibrary.org/obo/UO_0000008">
        <rdf:type rdf:resource="http://purl.obolibrary.org/obo/UO_0000001"/>
        <obo:IAO_0000111>meter</obo:IAO_0000111>
        <obo:IAO_0000412 rdf:resource="http://purl.obolibrary.org/obo/uo.owl"/>
        <rdfs:comment>&quot;A length unit which is equal to the length of the path traveled by light in vacuum during a time interval of 1/299 792 458 of a second.&quot; [BIPM:BIPM, NIST:NIST]</rdfs:comment>
        <rdfs:label>meter</rdfs:label>
        <oboInOwl:hasExactSynonym>m</oboInOwl:hasExactSynonym>
        <oboInOwl:hasExactSynonym>metre</oboInOwl:hasExactSynonym>
    </owl:NamedIndividual>
    


    <!-- http://purl.obolibrary.org/obo/UO_0000009 -->

    <owl:NamedIndividual rdf:about="http://purl.obolibrary.org/obo/UO_0000009">
        <rdf:type rdf:resource="http://purl.obolibrary.org/obo/UO_0000002"/>
        <obo:IAO_0000111>kilogram</obo:IAO_0000111>
        <obo:IAO_0000412 rdf:resource="http://purl.obolibrary.org/obo/uo.owl"/>
        <rdfs:comment>&quot;A mass unit which is equal to the mass of the International Prototype Kilogram kept by the BIPM at Svres, France.&quot; [BIPM:BIPM, NIST:NIST]</rdfs:comment>
        <rdfs:label>kilogram</rdfs:label>
        <oboInOwl:hasExactSynonym>kg</oboInOwl:hasExactSynonym>
    </owl:NamedIndividual>
    


    <!-- http://purl.obolibrary.org/obo/UO_0000010 -->

    <owl:NamedIndividual rdf:about="http://purl.obolibrary.org/obo/UO_0000010">
        <rdf:type rdf:resource="http://purl.obolibrary.org/obo/UO_0000003"/>
        <obo:IAO_0000111>second</obo:IAO_0000111>
        <obo:IAO_0000412 rdf:resource="http://purl.obolibrary.org/obo/uo.owl"/>
        <rdfs:comment>&quot;A time unit which is equal to the duration of 9 192 631 770 periods of the radiation corresponding to the transition between the two hyperfine levels of the ground state of the caesium 133 atom.&quot; [BIPM:BIPM, NIST:NIST]</rdfs:comment>
        <rdfs:label>second</rdfs:label>
        <oboInOwl:hasExactSynonym>s</oboInOwl:hasExactSynonym>
    </owl:NamedIndividual>
    


    <!-- http://purl.obolibrary.org/obo/UO_0000015 -->

    <owl:NamedIndividual rdf:about="http://purl.obolibrary.org/obo/UO_0000015">
        <rdf:type rdf:resource="http://purl.obolibrary.org/obo/UO_0000001"/>
        <obo:IAO_0000111>centimeter</obo:IAO_0000111>
        <obo:IAO_0000412 rdf:resource="http://purl.obolibrary.org/obo/uo.owl"/>
        <rdfs:comment>&quot;A length unit which is equal to one hundredth of a meter or 10^[-2] m.&quot; [NIST:NIST]</rdfs:comment>
        <rdfs:label>centimeter</rdfs:label>
        <oboInOwl:hasExactSynonym>centimetre</oboInOwl:hasExactSynonym>
        <oboInOwl:hasExactSynonym>cm</oboInOwl:hasExactSynonym>
    </owl:NamedIndividual>
    


    <!-- http://purl.obolibrary.org/obo/UO_0000016 -->

    <owl:NamedIndividual rdf:about="http://purl.obolibrary.org/obo/UO_0000016">
        <rdf:type rdf:resource="http://purl.obolibrary.org/obo/UO_0000001"/>
        <obo:IAO_0000111>millimeter</obo:IAO_0000111>
        <obo:IAO_0000412 rdf:resource="http://purl.obolibrary.org/obo/uo.owl"/>
        <rdfs:comment>&quot;A length unit which is equal to one thousandth of a meter or 10^[-3] m.&quot; [NIST:NIST]</rdfs:comment>
        <rdfs:label>millimeter</rdfs:label>
        <oboInOwl:hasExactSynonym>micrometre</oboInOwl:hasExactSynonym>
        <oboInOwl:hasExactSynonym>mm</oboInOwl:hasExactSynonym>
    </owl:NamedIndividual>
    


    <!-- http://purl.obolibrary.org/obo/UO_0000017 -->

    <owl:NamedIndividual rdf:about="http://purl.obolibrary.org/obo/UO_0000017">
        <rdf:type rdf:resource="http://purl.obolibrary.org/obo/UO_0000001"/>
        <obo:IAO_0000111>micrometer</obo:IAO_0000111>
        <obo:IAO_0000412 rdf:resource="http://purl.obolibrary.org/obo/uo.owl"/>
        <rdfs:comment>&quot;A length unit which is equal to one millionth of a meter or 10^[-6] m.&quot; [NIST:NIST]</rdfs:comment>
        <rdfs:label>micrometer</rdfs:label>
        <oboInOwl:hasExactSynonym>micrometre</oboInOwl:hasExactSynonym>
        <oboInOwl:hasExactSynonym>micron</oboInOwl:hasExactSynonym>
        <oboInOwl:hasExactSynonym>um</oboInOwl:hasExactSynonym>
    </owl:NamedIndividual>
    


    <!-- http://purl.obolibrary.org/obo/UO_0000018 -->

    <owl:NamedIndividual rdf:about="http://purl.obolibrary.org/obo/UO_0000018">
        <rdf:type rdf:resource="http://purl.obolibrary.org/obo/UO_0000001"/>
        <obo:IAO_0000111>nanometer</obo:IAO_0000111>
        <obo:IAO_0000412 rdf:resource="http://purl.obolibrary.org/obo/uo.owl"/>
        <rdfs:comment>&quot;A length unit which is equal to one thousandth of one millionth of a meter or 10^[-9] m.&quot; [NIST:NIST]</rdfs:comment>
        <rdfs:label>nanometer</rdfs:label>
        <oboInOwl:hasExactSynonym>nanometre</oboInOwl:hasExactSynonym>
        <oboInOwl:hasExactSynonym>nm</oboInOwl:hasExactSynonym>
    </owl:NamedIndividual>
    


    <!-- http://purl.obolibrary.org/obo/UO_0000019 -->

    <owl:NamedIndividual rdf:about="http://purl.obolibrary.org/obo/UO_0000019">
        <rdf:type rdf:resource="http://purl.obolibrary.org/obo/UO_0000001"/>
        <obo:IAO_0000111>angstrom</obo:IAO_0000111>
        <obo:IAO_0000412 rdf:resource="http://purl.obolibrary.org/obo/uo.owl"/>
        <rdfs:comment>&quot;A length unit which is equal to 10 [-10] m.&quot; [NIST:NIST]</rdfs:comment>
        <rdfs:label>angstrom</rdfs:label>
        <oboInOwl:hasExactSynonym>Ã…</oboInOwl:hasExactSynonym>
    </owl:NamedIndividual>
    


    <!-- http://purl.obolibrary.org/obo/UO_0000021 -->

    <owl:NamedIndividual rdf:about="http://purl.obolibrary.org/obo/UO_0000021">
        <rdf:type rdf:resource="http://purl.obolibrary.org/obo/UO_0000002"/>
        <obo:IAO_0000111>gram</obo:IAO_0000111>
        <obo:IAO_0000412 rdf:resource="http://purl.obolibrary.org/obo/uo.owl"/>
        <rdfs:comment>&quot;A mass unit which is equal to one thousandth of a kilogram or 10^[-3] kg.&quot; [NIST:NIST]</rdfs:comment>
        <rdfs:label>gram</rdfs:label>
        <oboInOwl:hasExactSynonym>g</oboInOwl:hasExactSynonym>
    </owl:NamedIndividual>
    


    <!-- http://purl.obolibrary.org/obo/UO_0000022 -->

    <owl:NamedIndividual rdf:about="http://purl.obolibrary.org/obo/UO_0000022">
        <rdf:type rdf:resource="http://purl.obolibrary.org/obo/UO_0000002"/>
        <obo:IAO_0000111>milligram</obo:IAO_0000111>
        <obo:IAO_0000412 rdf:resource="http://purl.obolibrary.org/obo/uo.owl"/>
        <rdfs:comment>&quot;A mass unit which is equal to one thousandth of a gram or 10^[-3] g.&quot; [UOC:GVG]</rdfs:comment>
        <rdfs:label>milligram</rdfs:label>
        <oboInOwl:hasExactSynonym>mg</oboInOwl:hasExactSynonym>
    </owl:NamedIndividual>
    


    <!-- http://purl.obolibrary.org/obo/UO_0000023 -->

    <owl:NamedIndividual rdf:about="http://purl.obolibrary.org/obo/UO_0000023">
        <rdf:type rdf:resource="http://purl.obolibrary.org/obo/UO_0000002"/>
        <obo:IAO_0000111>microgram</obo:IAO_0000111>
        <obo:IAO_0000412 rdf:resource="http://purl.obolibrary.org/obo/uo.owl"/>
        <rdfs:comment>&quot;A mass unit which is equal to one millionth of a gram or 10^[-6] g.&quot; [UOC:GVG]</rdfs:comment>
        <rdfs:label>microgram</rdfs:label>
        <oboInOwl:hasExactSynonym>ug</oboInOwl:hasExactSynonym>
    </owl:NamedIndividual>
    


    <!-- http://purl.obolibrary.org/obo/UO_0000024 -->

    <owl:NamedIndividual rdf:about="http://purl.obolibrary.org/obo/UO_0000024">
        <rdf:type rdf:resource="http://purl.obolibrary.org/obo/UO_0000002"/>
        <obo:IAO_0000111>nanogram</obo:IAO_0000111>
        <obo:IAO_0000412 rdf:resource="http://purl.obolibrary.org/obo/uo.owl"/>
        <rdfs:comment>&quot;A mass unit which is equal to one thousandth of one millionth of a gram or 10^[-9] g.&quot; [UOC:GVG]</rdfs:comment>
        <rdfs:label>nanogram</rdfs:label>
        <oboInOwl:hasExactSynonym>ng</oboInOwl:hasExactSynonym>
    </owl:NamedIndividual>
    


    <!-- http://purl.obolibrary.org/obo/UO_0000025 -->

    <owl:NamedIndividual rdf:about="http://purl.obolibrary.org/obo/UO_0000025">
        <rdf:type rdf:resource="http://purl.obolibrary.org/obo/UO_0000002"/>
        <obo:IAO_0000111>picogram</obo:IAO_0000111>
        <obo:IAO_0000412 rdf:resource="http://purl.obolibrary.org/obo/uo.owl"/>
        <rdfs:comment>&quot;A mass unit which is equal to 10^[-12] g.&quot; [UOC:GVG]</rdfs:comment>
        <rdfs:label>picogram</rdfs:label>
        <oboInOwl:hasExactSynonym>pg</oboInOwl:hasExactSynonym>
    </owl:NamedIndividual>
    


    <!-- http://purl.obolibrary.org/obo/UO_0000027 -->

    <owl:NamedIndividual rdf:about="http://purl.obolibrary.org/obo/UO_0000027">
        <rdf:type rdf:resource="http://purl.obolibrary.org/obo/UO_0000005"/>
        <obo:IAO_0000111>degree Celsius</obo:IAO_0000111>
        <obo:IAO_0000412 rdf:resource="http://purl.obolibrary.org/obo/uo.owl"/>
        <rdfs:comment>&quot;A temperature unit which is equal to one kelvin degree. However, they have their zeros at different points. The centigrade scale has its zero at 273.15 K.&quot; [NIST:NIST]</rdfs:comment>
        <rdfs:label>degree Celsius</rdfs:label>
        <oboInOwl:hasExactSynonym>C</oboInOwl:hasExactSynonym>
    </owl:NamedIndividual>
    


    <!-- http://purl.obolibrary.org/obo/UO_0000031 -->

    <owl:NamedIndividual rdf:about="http://purl.obolibrary.org/obo/UO_0000031">
        <rdf:type rdf:resource="http://purl.obolibrary.org/obo/UO_0000003"/>
        <obo:IAO_0000111>minute</obo:IAO_0000111>
        <obo:IAO_0000412 rdf:resource="http://purl.obolibrary.org/obo/uo.owl"/>
        <rdfs:comment>&quot;A time unit which is equal to 60 seconds.&quot; [Wikipedia:Wikipedia]</rdfs:comment>
        <rdfs:label>minute</rdfs:label>
        <oboInOwl:hasExactSynonym>min</oboInOwl:hasExactSynonym>
    </owl:NamedIndividual>
    


    <!-- http://purl.obolibrary.org/obo/UO_0000032 -->

    <owl:NamedIndividual rdf:about="http://purl.obolibrary.org/obo/UO_0000032">
        <rdf:type rdf:resource="http://purl.obolibrary.org/obo/UO_0000003"/>
        <obo:IAO_0000111>hour</obo:IAO_0000111>
        <obo:IAO_0000412 rdf:resource="http://purl.obolibrary.org/obo/uo.owl"/>
        <rdfs:comment>&quot;A time unit which is equal to 3600 seconds or 60 minutes.&quot; [Wikipedia:Wikipedia]</rdfs:comment>
        <rdfs:label>hour</rdfs:label>
        <oboInOwl:hasExactSynonym>h</oboInOwl:hasExactSynonym>
    </owl:NamedIndividual>
    


    <!-- http://purl.obolibrary.org/obo/UO_0000033 -->

    <owl:NamedIndividual rdf:about="http://purl.obolibrary.org/obo/UO_0000033">
        <rdf:type rdf:resource="http://purl.obolibrary.org/obo/UO_0000003"/>
        <obo:IAO_0000111>day</obo:IAO_0000111>
        <obo:IAO_0000412 rdf:resource="http://purl.obolibrary.org/obo/uo.owl"/>
        <rdfs:comment>&quot;A time unit which is equal to 24 hours.&quot; [Wikipedia:Wikipedia]</rdfs:comment>
        <rdfs:label>day</rdfs:label>
    </owl:NamedIndividual>
    


    <!-- http://purl.obolibrary.org/obo/UO_0000034 -->

    <owl:NamedIndividual rdf:about="http://purl.obolibrary.org/obo/UO_0000034">
        <rdf:type rdf:resource="http://purl.obolibrary.org/obo/UO_0000003"/>
        <obo:IAO_0000111>week</obo:IAO_0000111>
        <obo:IAO_0000412 rdf:resource="http://purl.obolibrary.org/obo/uo.owl"/>
        <rdfs:comment>&quot;A time unit which is equal to 7 days.&quot; [Wikipedia:Wikipedia]</rdfs:comment>
        <rdfs:label>week</rdfs:label>
    </owl:NamedIndividual>
    


    <!-- http://purl.obolibrary.org/obo/UO_0000035 -->

    <owl:NamedIndividual rdf:about="http://purl.obolibrary.org/obo/UO_0000035">
        <rdf:type rdf:resource="http://purl.obolibrary.org/obo/UO_0000003"/>
        <obo:IAO_0000111>month</obo:IAO_0000111>
        <obo:IAO_0000412 rdf:resource="http://purl.obolibrary.org/obo/uo.owl"/>
        <rdfs:comment>&quot;A time unit which is approximately equal to the length of time of one of cycle of the moon&apos;s phases which in science is taken to be equal to 30 days.&quot; [Wikipedia:Wikipedia]</rdfs:comment>
        <rdfs:label>month</rdfs:label>
    </owl:NamedIndividual>
    


    <!-- http://purl.obolibrary.org/obo/UO_0000036 -->

    <owl:NamedIndividual rdf:about="http://purl.obolibrary.org/obo/UO_0000036">
        <rdf:type rdf:resource="http://purl.obolibrary.org/obo/UO_0000003"/>
        <obo:IAO_0000111>year</obo:IAO_0000111>
        <obo:IAO_0000412 rdf:resource="http://purl.obolibrary.org/obo/uo.owl"/>
        <rdfs:comment>&quot;A time unit which is equal to 12 months which in science is taken to be equal to 365.25 days.&quot; [Wikipedia:Wikipedia]</rdfs:comment>
        <rdfs:label>year</rdfs:label>
    </owl:NamedIndividual>
    


    <!-- http://purl.obolibrary.org/obo/UO_0000039 -->

    <owl:NamedIndividual rdf:about="http://purl.obolibrary.org/obo/UO_0000039">
        <rdf:type rdf:resource="http://purl.obolibrary.org/obo/UO_0000006"/>
        <obo:IAO_0000111>micromole</obo:IAO_0000111>
        <obo:IAO_0000412 rdf:resource="http://purl.obolibrary.org/obo/uo.owl"/>
        <rdfs:comment>&quot;A substance unit equal to a millionth of a mol or 10^[-6] mol.&quot; [NIST:NIST]</rdfs:comment>
        <rdfs:label>micromole</rdfs:label>
        <oboInOwl:hasExactSynonym>umol</oboInOwl:hasExactSynonym>
    </owl:NamedIndividual>
    


    <!-- http://purl.obolibrary.org/obo/UO_0000041 -->

    <owl:NamedIndividual rdf:about="http://purl.obolibrary.org/obo/UO_0000041">
        <rdf:type rdf:resource="http://purl.obolibrary.org/obo/UO_0000006"/>
        <obo:IAO_0000111>nanomole</obo:IAO_0000111>
        <obo:IAO_0000412 rdf:resource="http://purl.obolibrary.org/obo/uo.owl"/>
        <rdfs:comment>&quot;A substance unit equal to one thousandth of one millionth of a mole or 10^[-9] mol.&quot; [NIST:NIST]</rdfs:comment>
        <rdfs:label>nanomole</rdfs:label>
        <oboInOwl:hasExactSynonym>nmol</oboInOwl:hasExactSynonym>
    </owl:NamedIndividual>
    


    <!-- http://purl.obolibrary.org/obo/UO_0000042 -->

    <owl:NamedIndividual rdf:about="http://purl.obolibrary.org/obo/UO_0000042">
        <rdf:type rdf:resource="http://purl.obolibrary.org/obo/UO_0000006"/>
        <obo:IAO_0000111>picomole</obo:IAO_0000111>
        <obo:IAO_0000412 rdf:resource="http://purl.obolibrary.org/obo/uo.owl"/>
        <rdfs:comment>&quot;A substance unit equal to 10^[-12] mol.&quot; [NIST:NIST]</rdfs:comment>
        <rdfs:label>picomole</rdfs:label>
        <oboInOwl:hasExactSynonym>pmol</oboInOwl:hasExactSynonym>
    </owl:NamedIndividual>
    


    <!-- http://purl.obolibrary.org/obo/UO_0000062 -->

    <owl:NamedIndividual rdf:about="http://purl.obolibrary.org/obo/UO_0000062">
        <rdf:type rdf:resource="http://purl.obolibrary.org/obo/UO_0000051"/>
        <obo:IAO_0000111>molar</obo:IAO_0000111>
        <obo:IAO_0000412 rdf:resource="http://purl.obolibrary.org/obo/uo.owl"/>
        <rdfs:comment>&quot;A unit of concentration which expresses a concentration of 1 mole of solute per liter of solution (mol/L).&quot; [UOC:GVG]</rdfs:comment>
        <rdfs:label>molar</rdfs:label>
        <oboInOwl:hasExactSynonym>M</oboInOwl:hasExactSynonym>
    </owl:NamedIndividual>
    


    <!-- http://purl.obolibrary.org/obo/UO_0000063 -->

    <owl:NamedIndividual rdf:about="http://purl.obolibrary.org/obo/UO_0000063">
        <rdf:type rdf:resource="http://purl.obolibrary.org/obo/UO_0000051"/>
        <obo:IAO_0000111>millimolar</obo:IAO_0000111>
        <obo:IAO_0000412 rdf:resource="http://purl.obolibrary.org/obo/uo.owl"/>
        <rdfs:comment>&quot;A unit of molarity which is equal to one thousandth of a molar or 10^[-3] M.&quot; [UOC:GVG]</rdfs:comment>
        <rdfs:label>millimolar</rdfs:label>
        <oboInOwl:hasExactSynonym>mM</oboInOwl:hasExactSynonym>
    </owl:NamedIndividual>
    


    <!-- http://purl.obolibrary.org/obo/UO_0000064 -->

    <owl:NamedIndividual rdf:about="http://purl.obolibrary.org/obo/UO_0000064">
        <rdf:type rdf:resource="http://purl.obolibrary.org/obo/UO_0000051"/>
        <obo:IAO_0000111>micromolar</obo:IAO_0000111>
        <obo:IAO_0000412 rdf:resource="http://purl.obolibrary.org/obo/uo.owl"/>
        <rdfs:comment>&quot;A unit of molarity which is equal to one millionth of a molar or 10^[-6] M.&quot; [UOC:GVG]</rdfs:comment>
        <rdfs:label>micromolar</rdfs:label>
        <oboInOwl:hasExactSynonym>uM</oboInOwl:hasExactSynonym>
    </owl:NamedIndividual>
    


    <!-- http://purl.obolibrary.org/obo/UO_0000065 -->

    <owl:NamedIndividual rdf:about="http://purl.obolibrary.org/obo/UO_0000065">
        <rdf:type rdf:resource="http://purl.obolibrary.org/obo/UO_0000051"/>
        <obo:IAO_0000111>nanomolar</obo:IAO_0000111>
        <obo:IAO_0000412 rdf:resource="http://purl.obolibrary.org/obo/uo.owl"/>
        <rdfs:comment>&quot;A unit of molarity which is equal to one thousandth of one millionth of a molar or 10^[-9] M.&quot; [UOC:GVG]</rdfs:comment>
        <rdfs:label>nanomolar</rdfs:label>
        <oboInOwl:hasExactSynonym>nM</oboInOwl:hasExactSynonym>
    </owl:NamedIndividual>
    


    <!-- http://purl.obolibrary.org/obo/UO_0000066 -->

    <owl:NamedIndividual rdf:about="http://purl.obolibrary.org/obo/UO_0000066">
        <rdf:type rdf:resource="http://purl.obolibrary.org/obo/UO_0000051"/>
        <obo:IAO_0000111>picomolar</obo:IAO_0000111>
        <obo:IAO_0000412 rdf:resource="http://purl.obolibrary.org/obo/uo.owl"/>
        <rdfs:comment>&quot;A unit of molarity which is equal to 10^[-12] M.&quot; [UOC:GVG]</rdfs:comment>
        <rdfs:label>picomolar</rdfs:label>
        <oboInOwl:hasExactSynonym>pM</oboInOwl:hasExactSynonym>
    </owl:NamedIndividual>
    


    <!-- http://purl.obolibrary.org/obo/UO_0000097 -->

    <owl:NamedIndividual rdf:about="http://purl.obolibrary.org/obo/UO_0000097">
        <rdf:type rdf:resource="http://purl.obolibrary.org/obo/UO_0000095"/>
        <obo:IAO_0000111>cubic centimeter</obo:IAO_0000111>
        <obo:IAO_0000412 rdf:resource="http://purl.obolibrary.org/obo/uo.owl"/>
        <rdfs:comment>&quot;A volume unit which is equal to one millionth of a cubic meter or 10^[-9] m^[3], or to 1 ml.&quot; [NIST:NIST]</rdfs:comment>
        <rdfs:label>cubic centimeter</rdfs:label>
        <oboInOwl:hasExactSynonym>cc</oboInOwl:hasExactSynonym>
        <oboInOwl:hasExactSynonym>cm^3</oboInOwl:hasExactSynonym>
        <oboInOwl:hasExactSynonym>cubic centimetre</oboInOwl:hasExactSynonym>
    </owl:NamedIndividual>
    


    <!-- http://purl.obolibrary.org/obo/UO_0000098 -->

    <owl:NamedIndividual rdf:about="http://purl.obolibrary.org/obo/UO_0000098">
        <rdf:type rdf:resource="http://purl.obolibrary.org/obo/UO_0000095"/>
        <obo:IAO_0000111>milliliter</obo:IAO_0000111>
        <obo:IAO_0000412 rdf:resource="http://purl.obolibrary.org/obo/uo.owl"/>
        <rdfs:comment>&quot;A volume unit which is equal to one thousandth of a liter or 10^[-3] L, or to 1 cubic centimeter.&quot; [NIST:NIST]</rdfs:comment>
        <rdfs:label>milliliter</rdfs:label>
        <oboInOwl:hasExactSynonym>millilitre</oboInOwl:hasExactSynonym>
        <oboInOwl:hasExactSynonym>ml</oboInOwl:hasExactSynonym>
    </owl:NamedIndividual>
    


    <!-- http://purl.obolibrary.org/obo/UO_0000099 -->

    <owl:NamedIndividual rdf:about="http://purl.obolibrary.org/obo/UO_0000099">
        <rdf:type rdf:resource="http://purl.obolibrary.org/obo/UO_0000095"/>
        <obo:IAO_0000111>liter</obo:IAO_0000111>
        <obo:IAO_0000412 rdf:resource="http://purl.obolibrary.org/obo/uo.owl"/>
        <rdfs:comment>&quot;A volume unit which is equal to one thousandth of a cubic meter or 10^[-3] m^[3], or to 1 decimeter.&quot; [NIST:NIST]</rdfs:comment>
        <rdfs:label>liter</rdfs:label>
        <oboInOwl:hasExactSynonym>L</oboInOwl:hasExactSynonym>
        <oboInOwl:hasExactSynonym>l</oboInOwl:hasExactSynonym>
        <oboInOwl:hasExactSynonym>litre</oboInOwl:hasExactSynonym>
    </owl:NamedIndividual>
    


    <!-- http://purl.obolibrary.org/obo/UO_0000100 -->

    <owl:NamedIndividual rdf:about="http://purl.obolibrary.org/obo/UO_0000100">
        <rdf:type rdf:resource="http://purl.obolibrary.org/obo/UO_0000095"/>
        <obo:IAO_0000111>cubic decimeter</obo:IAO_0000111>
        <obo:IAO_0000412 rdf:resource="http://purl.obolibrary.org/obo/uo.owl"/>
        <rdfs:comment>&quot;A volume unit which is equal to one thousand of a cubic meter or 10^[-3] m^[3], or to 1 L.&quot; [NIST:NIST]</rdfs:comment>
        <rdfs:label>cubic decimeter</rdfs:label>
        <oboInOwl:hasExactSynonym>cubic decimetre</oboInOwl:hasExactSynonym>
        <oboInOwl:hasExactSynonym>dm^[3]</oboInOwl:hasExactSynonym>
    </owl:NamedIndividual>
    


    <!-- http://purl.obolibrary.org/obo/UO_0000101 -->

    <owl:NamedIndividual rdf:about="http://purl.obolibrary.org/obo/UO_0000101">
        <rdf:type rdf:resource="http://purl.obolibrary.org/obo/UO_0000095"/>
        <obo:IAO_0000111>microliter</obo:IAO_0000111>
        <obo:IAO_0000412 rdf:resource="http://purl.obolibrary.org/obo/uo.owl"/>
        <rdfs:comment>&quot;A volume unit which is equal to one millionth of a liter or 10^[-6] L.&quot; [NIST:NIST]</rdfs:comment>
        <rdfs:label>microliter</rdfs:label>
        <oboInOwl:hasExactSynonym>microlitre</oboInOwl:hasExactSynonym>
        <oboInOwl:hasExactSynonym>ul</oboInOwl:hasExactSynonym>
    </owl:NamedIndividual>
    


    <!-- http://purl.obolibrary.org/obo/UO_0000102 -->

    <owl:NamedIndividual rdf:about="http://purl.obolibrary.org/obo/UO_0000102">
        <rdf:type rdf:resource="http://purl.obolibrary.org/obo/UO_0000095"/>
        <obo:IAO_0000111>nanoliter</obo:IAO_0000111>
        <obo:IAO_0000412 rdf:resource="http://purl.obolibrary.org/obo/uo.owl"/>
        <rdfs:comment>&quot;A volume unit which is equal to one thousandth of one millionth of a liter or 10^[-9] L.&quot; [NIST:NIST]</rdfs:comment>
        <rdfs:label>nanoliter</rdfs:label>
        <oboInOwl:hasExactSynonym>nanolitre</oboInOwl:hasExactSynonym>
        <oboInOwl:hasExactSynonym>nl</oboInOwl:hasExactSynonym>
    </owl:NamedIndividual>
    


    <!-- http://purl.obolibrary.org/obo/UO_0000103 -->

    <owl:NamedIndividual rdf:about="http://purl.obolibrary.org/obo/UO_0000103">
        <rdf:type rdf:resource="http://purl.obolibrary.org/obo/UO_0000095"/>
        <obo:IAO_0000111>picoliter</obo:IAO_0000111>
        <obo:IAO_0000412 rdf:resource="http://purl.obolibrary.org/obo/uo.owl"/>
        <rdfs:comment>&quot;A volume unit which is equal to 10^[-12] L.&quot; [NIST:NIST]</rdfs:comment>
        <rdfs:label>picoliter</rdfs:label>
        <oboInOwl:hasExactSynonym>picolitre</oboInOwl:hasExactSynonym>
        <oboInOwl:hasExactSynonym>pl</oboInOwl:hasExactSynonym>
    </owl:NamedIndividual>
    


    <!-- http://purl.obolibrary.org/obo/UO_0000106 -->

    <owl:NamedIndividual rdf:about="http://purl.obolibrary.org/obo/UO_0000106">
        <rdf:type rdf:resource="http://purl.obolibrary.org/obo/UO_0000105"/>
        <obo:IAO_0000111>hertz</obo:IAO_0000111>
        <obo:IAO_0000412 rdf:resource="http://purl.obolibrary.org/obo/uo.owl"/>
        <rdfs:comment>&quot;A frequency unit which is equal to 1 complete cycle of a recurring phenomenon in 1 second.&quot; [NIST:NIST]</rdfs:comment>
        <rdfs:label>hertz</rdfs:label>
        <oboInOwl:hasExactSynonym>Hz</oboInOwl:hasExactSynonym>
        <oboInOwl:hasExactSynonym>s^1</oboInOwl:hasExactSynonym>
    </owl:NamedIndividual>
    


    <!-- http://purl.obolibrary.org/obo/UO_0000163 -->

    <owl:NamedIndividual rdf:about="http://purl.obolibrary.org/obo/UO_0000163">
        <rdf:type rdf:resource="http://purl.obolibrary.org/obo/UO_0000051"/>
        <obo:IAO_0000111>mass percentage</obo:IAO_0000111>
        <obo:IAO_0000412 rdf:resource="http://purl.obolibrary.org/obo/uo.owl"/>
        <rdfs:comment>&quot;A dimensionless concentration unit which denotes the mass of a substance in a mixture as a percentage of the mass of the entire mixture.&quot; [Wikipedia:Wikipedia]</rdfs:comment>
        <rdfs:label>mass percentage</rdfs:label>
        <oboInOwl:hasExactSynonym>w/w</oboInOwl:hasExactSynonym>
        <oboInOwl:hasExactSynonym>weight-weight percentage</oboInOwl:hasExactSynonym>
    </owl:NamedIndividual>
    


    <!-- http://purl.obolibrary.org/obo/UO_0000164 -->

    <owl:NamedIndividual rdf:about="http://purl.obolibrary.org/obo/UO_0000164">
        <rdf:type rdf:resource="http://purl.obolibrary.org/obo/UO_0000051"/>
        <obo:IAO_0000111>mass volume percentage</obo:IAO_0000111>
        <obo:IAO_0000412 rdf:resource="http://purl.obolibrary.org/obo/uo.owl"/>
        <rdfs:comment>&quot;A dimensionless concentration unit which denotes the mass of the substance in a mixture as a percentage of the volume of the entire mixture.&quot; [UOC:GVG]</rdfs:comment>
        <rdfs:label>mass volume percentage</rdfs:label>
        <oboInOwl:hasExactSynonym>(w/v)</oboInOwl:hasExactSynonym>
        <oboInOwl:hasExactSynonym>weight-volume percentage</oboInOwl:hasExactSynonym>
    </owl:NamedIndividual>
    


    <!-- http://purl.obolibrary.org/obo/UO_0000165 -->

    <owl:NamedIndividual rdf:about="http://purl.obolibrary.org/obo/UO_0000165">
        <rdf:type rdf:resource="http://purl.obolibrary.org/obo/UO_0000051"/>
        <obo:IAO_0000111>volume percentage</obo:IAO_0000111>
        <obo:IAO_0000412 rdf:resource="http://purl.obolibrary.org/obo/uo.owl"/>
        <rdfs:comment>&quot;A dimensionless concentration unit which denotes the volume of the solute in mL per 100 mL of the resulting solution.&quot; [UOC:GVG]</rdfs:comment>
        <rdfs:label>volume percentage</rdfs:label>
        <oboInOwl:hasExactSynonym>% (v/v)</oboInOwl:hasExactSynonym>
    </owl:NamedIndividual>
    


    <!-- http://purl.obolibrary.org/obo/UO_0000175 -->

    <owl:NamedIndividual rdf:about="http://purl.obolibrary.org/obo/UO_0000175">
        <rdf:type rdf:resource="http://purl.obolibrary.org/obo/UO_0000051"/>
        <obo:IAO_0000111>gram per liter</obo:IAO_0000111>
        <obo:IAO_0000412 rdf:resource="http://purl.obolibrary.org/obo/uo.owl"/>
        <rdfs:comment>&quot;A mass unit density which is equal to mass of an object in grams divided by the volume in liters.&quot; [UOC:GVG]</rdfs:comment>
        <rdfs:label>gram per liter</rdfs:label>
        <oboInOwl:hasExactSynonym>g/L</oboInOwl:hasExactSynonym>
        <oboInOwl:hasExactSynonym>gram per litre</oboInOwl:hasExactSynonym>
    </owl:NamedIndividual>
    


    <!-- http://purl.obolibrary.org/obo/UO_0000176 -->

    <owl:NamedIndividual rdf:about="http://purl.obolibrary.org/obo/UO_0000176">
        <rdf:type rdf:resource="http://purl.obolibrary.org/obo/UO_0000051"/>
        <obo:IAO_0000111>milligram per milliliter</obo:IAO_0000111>
        <obo:IAO_0000412 rdf:resource="http://purl.obolibrary.org/obo/uo.owl"/>
        <rdfs:comment>&quot;A mass unit density which is equal to mass of an object in milligrams divided by the volume in milliliters.&quot; [UOC:GVG]</rdfs:comment>
        <rdfs:label>milligram per milliliter</rdfs:label>
        <oboInOwl:hasExactSynonym>mg/ml</oboInOwl:hasExactSynonym>
        <oboInOwl:hasExactSynonym>milligram per millilitre</oboInOwl:hasExactSynonym>
    </owl:NamedIndividual>
    


    <!-- http://purl.obolibrary.org/obo/UO_0000195 -->

    <owl:NamedIndividual rdf:about="http://purl.obolibrary.org/obo/UO_0000195">
        <rdf:type rdf:resource="http://purl.obolibrary.org/obo/UO_0000005"/>
        <obo:IAO_0000111>degree Fahrenheit</obo:IAO_0000111>
        <obo:IAO_0000412 rdf:resource="http://purl.obolibrary.org/obo/uo.owl"/>
        <rdfs:comment>&quot;A temperature unit which is equal to 5/9ths of a kelvin. Negative 40 degrees Fahrenheit is equal to negative 40 degrees Celsius.&quot; [Wikipedia:Wikipedia]</rdfs:comment>
        <rdfs:label>degree Fahrenheit</rdfs:label>
        <oboInOwl:hasExactSynonym>F</oboInOwl:hasExactSynonym>
    </owl:NamedIndividual>
    


    <!-- http://purl.obolibrary.org/obo/UO_0000196 -->

    <owl:NamedIndividual rdf:about="http://purl.obolibrary.org/obo/UO_0000196">
        <rdf:type rdf:resource="http://purl.obolibrary.org/obo/UO_0000051"/>
        <obo:IAO_0000111>pH</obo:IAO_0000111>
        <obo:IAO_0000412 rdf:resource="http://purl.obolibrary.org/obo/uo.owl"/>
        <rdfs:comment>&quot;A dimensionless concentration notation which denotes the acidity of a solution in terms of activity of hydrogen ions (H+).&quot; [Wikipedia:Wikipedia]</rdfs:comment>
        <rdfs:label>pH</rdfs:label>
    </owl:NamedIndividual>
    


    <!-- http://purl.obolibrary.org/obo/UO_0000207 -->

    <owl:NamedIndividual rdf:about="http://purl.obolibrary.org/obo/UO_0000207">
        <rdf:type rdf:resource="http://purl.obolibrary.org/obo/UO_0000051"/>
        <obo:IAO_0000111>milliliter per liter</obo:IAO_0000111>
        <obo:IAO_0000412 rdf:resource="http://purl.obolibrary.org/obo/uo.owl"/>
        <rdfs:comment>&quot;A volume per unit volume unit which is equal to one millionth of a liter of solute in one liter of solution.&quot; [NIST:NIST]</rdfs:comment>
        <rdfs:label>milliliter per liter</rdfs:label>
        <oboInOwl:hasExactSynonym>millilitre per litre</oboInOwl:hasExactSynonym>
        <oboInOwl:hasExactSynonym>ml/l</oboInOwl:hasExactSynonym>
    </owl:NamedIndividual>
    


    <!-- http://purl.obolibrary.org/obo/UO_0000208 -->

    <owl:NamedIndividual rdf:about="http://purl.obolibrary.org/obo/UO_0000208">
        <rdf:type rdf:resource="http://purl.obolibrary.org/obo/UO_0000051"/>
        <obo:IAO_0000111>gram per deciliter</obo:IAO_0000111>
        <obo:IAO_0000412 rdf:resource="http://purl.obolibrary.org/obo/uo.owl"/>
        <rdfs:comment>&quot;A mass density unit which is equal to mass of an object in grams divided by the volume in deciliters.&quot; [UOC:GVG]</rdfs:comment>
        <rdfs:label>gram per deciliter</rdfs:label>
        <oboInOwl:hasExactSynonym>g/dl</oboInOwl:hasExactSynonym>
        <oboInOwl:hasExactSynonym>gram per decilitre</oboInOwl:hasExactSynonym>
    </owl:NamedIndividual>
    


    <!-- http://purl.obolibrary.org/obo/UO_0000271 -->

    <owl:NamedIndividual rdf:about="http://purl.obolibrary.org/obo/UO_0000271">
        <rdf:type rdf:resource="http://purl.obolibrary.org/obo/UO_0000270"/>
        <obo:IAO_0000111>microliters per minute</obo:IAO_0000111>
        <obo:IAO_0000412 rdf:resource="http://purl.obolibrary.org/obo/uo.owl"/>
        <rdfs:comment>&quot;A volumetric flow rate unit which is equal to one microliter volume through a given surface in one minute.&quot; [UOC:GVG]</rdfs:comment>
        <rdfs:label>microliters per minute</rdfs:label>
        <oboInOwl:hasExactSynonym>microlitres per minute</oboInOwl:hasExactSynonym>
        <oboInOwl:hasExactSynonym>uL/min</oboInOwl:hasExactSynonym>
    </owl:NamedIndividual>
    


    <!-- http://purl.obolibrary.org/obo/UO_0000281 -->

    <owl:NamedIndividual rdf:about="http://purl.obolibrary.org/obo/UO_0000281">
        <rdf:type rdf:resource="http://purl.obolibrary.org/obo/UO_0000280"/>
        <obo:IAO_0000111>count per nanomolar second</obo:IAO_0000111>
        <obo:IAO_0000412 rdf:resource="http://purl.obolibrary.org/obo/uo.owl"/>
        <rdfs:comment>&quot;A rate unit which is equal to one over one nanomolar second.&quot; [UOC:GVG]</rdfs:comment>
        <rdfs:label>count per nanomolar second</rdfs:label>
        <oboInOwl:hasExactSynonym>nM^-1 s^-1</oboInOwl:hasExactSynonym>
    </owl:NamedIndividual>
    


    <!-- http://purl.obolibrary.org/obo/UO_0000282 -->

    <owl:NamedIndividual rdf:about="http://purl.obolibrary.org/obo/UO_0000282">
        <rdf:type rdf:resource="http://purl.obolibrary.org/obo/UO_0000280"/>
        <obo:IAO_0000111>count per molar second</obo:IAO_0000111>
        <obo:IAO_0000412 rdf:resource="http://purl.obolibrary.org/obo/uo.owl"/>
        <rdfs:comment>&quot;A rate unit which is equal to one over one molar second.&quot; [UOC:GVG]</rdfs:comment>
        <rdfs:label>count per molar second</rdfs:label>
        <oboInOwl:hasExactSynonym>M^-1 s^-1</oboInOwl:hasExactSynonym>
    </owl:NamedIndividual>
    


    <!-- http://purl.obolibrary.org/obo/UO_0000284 -->

    <owl:NamedIndividual rdf:about="http://purl.obolibrary.org/obo/UO_0000284">
        <rdf:type rdf:resource="http://purl.obolibrary.org/obo/UO_0000280"/>
        <obo:IAO_0000111>count per nanomolar</obo:IAO_0000111>
        <obo:IAO_0000412 rdf:resource="http://purl.obolibrary.org/obo/uo.owl"/>
        <rdfs:comment>&quot;A rate unit which is equal to one over one nanomolar.&quot; [UO:GVG]</rdfs:comment>
        <rdfs:label>count per nanomolar</rdfs:label>
        <oboInOwl:hasExactSynonym>1/nM</oboInOwl:hasExactSynonym>
        <oboInOwl:hasExactSynonym>nM^-1</oboInOwl:hasExactSynonym>
    </owl:NamedIndividual>
    


    <!-- http://purl.obolibrary.org/obo/UO_0000285 -->

    <owl:NamedIndividual rdf:about="http://purl.obolibrary.org/obo/UO_0000285">
        <rdf:type rdf:resource="http://purl.obolibrary.org/obo/UO_0000280"/>
        <obo:IAO_0000111>count per molar</obo:IAO_0000111>
        <obo:IAO_0000412 rdf:resource="http://purl.obolibrary.org/obo/uo.owl"/>
        <rdfs:comment>&quot;A rate unit which is equal to one over one molar.&quot; [UO:GVG]</rdfs:comment>
        <rdfs:label>count per molar</rdfs:label>
        <oboInOwl:hasExactSynonym>1/M</oboInOwl:hasExactSynonym>
        <oboInOwl:hasExactSynonym>M^-1</oboInOwl:hasExactSynonym>
    </owl:NamedIndividual>
    


    <!-- http://purl.obolibrary.org/obo/UO_0000301 -->

    <owl:NamedIndividual rdf:about="http://purl.obolibrary.org/obo/UO_0000301">
        <rdf:type rdf:resource="http://purl.obolibrary.org/obo/UO_0000051"/>
        <obo:IAO_0000111>microgram per liter</obo:IAO_0000111>
        <obo:IAO_0000412 rdf:resource="http://purl.obolibrary.org/obo/uo.owl"/>
        <rdfs:comment>&quot;A mass unit density which is equal to mass of an object in micrograms divided by the volume in liters.&quot; [UOC:GVG]</rdfs:comment>
        <rdfs:label>microgram per liter</rdfs:label>
        <oboInOwl:hasExactSynonym>microgram per litre</oboInOwl:hasExactSynonym>
        <oboInOwl:hasExactSynonym>ug/L</oboInOwl:hasExactSynonym>
    </owl:NamedIndividual>
</rdf:RDF>



<!-- Generated by the OWL API (version 4.5.6) https://github.com/owlcs/owlapi -->

